git/opencompl/lean-mlir/MLIR/MLIRParser.lean
@@ -1,6 +1,7 @@
 import MLIR.AST
 import MLIR.Doc
 import MLIR.P
+import MLIR.Dialects.BuiltinModel
 
 open MLIR.AST
 open MLIR.Doc
@@ -8,8 +9,13 @@ open MLIR.P
 
 
 namespace MLIR.MLIRParser
+
+-- We can parse any dialect at least as large as builtin
+section
+variable {α σ ε} [δ: Dialect α σ ε] [CoeDialect builtin δ]
+
 -- | ^ <name>
-def pbbname : P BBName := do 
+def pbbname : P BBName := do
   pconsume '^'
   let name <- pident
    return (BBName.mk name)
@@ -25,11 +31,11 @@ partial def pssaval : P SSAVal := do
 mutual
 
 -- | mh, needs to be mutual. Let's see if LEAN lets me do this.
-partial def pregion (u: Unit) : P Region :=  do
+partial def pregion (u: Unit) : P (Region δ) :=  do
   pconsume '{'
   -- HACK: entry block need not print block header. See: examples/region-with-no-args.mlir
   let b <- (if (<- ppeek? '^')
-           then pblock u 
+           then pblock u
            else pentryblock_no_label u)
 
   let bs <- (if (<- ppeek? '^')
@@ -42,37 +48,37 @@ partial def pregion (u: Unit) : P Region :=  do
 partial def pdim : P Dimension := do
   if (<- ppeek? '?')
   then return Dimension.Unknown
-  else do 
+  else do
     let sz <- pnat
     return Dimension.Known sz
 
-partial def ptype_vector : P MLIRTy := do
+partial def ptype_vector : P (MLIRType builtin) := do
   pident? "vector"
   pconsume '<'
-  let sz <- pnumber
+  let sz <- pnat
   pconsume 'x'
   let ty <- ptype ()
   pconsume '>'
-  return MLIRTy.vector [sz] [] ty
+  return builtin.vector [sz] [] ty
 
--- !<ident>.<ident>  
+-- !<ident>.<ident>
 partial def puser (u: Unit): P MLIRTy := do
     pconsume '!'
     let dialect <- pident
     pconsume '.'
     let ty <- pident
-    return MLIRTy.user (dialect ++ "." ++ ty)
+    return MLIRType.undefined (dialect ++ "." ++ ty)
 
 partial def ptype (u: Unit) : P MLIRTy := do
   eat_whitespace
   let dom <- (match (<- ppeek) with
              | some '(' => do
                 let args <- pintercalated '(' (ptype u) ',' ')'
-                return MLIRTy.tuple args
+                return MLIRType.tuple args
              | some 'i' => do
                  pconsume 'i'
                  let num <- pnumber
-                 return MLIRTy.int num
+                 return MLIRType.int num
              | some '!' => do
                   puser ()
              | other => do
@@ -83,7 +89,7 @@ partial def ptype (u: Unit) : P MLIRTy := do
         pconsume '-'
         pconsume '>' -- consume arrow
         let codom <- (ptype u)
-        return MLIRTy.fn dom codom
+        return MLIRType.fn dom codom
   | false => do
      return dom
 
@@ -101,39 +107,39 @@ partial def pattrvalue_int : P AttrVal := do
   let num <- pnumber
   pconsume ':'
   let ty <- ptype ()
-  return AttrVal.int num ty
+  return AttrValue.int num ty
 
 partial def ptensorelem (u: Unit): P TensorElem := do
   if (<- ppeek? '[') then
     let ts <- pintercalated '[' (ptensorelem ()) ','  ']'
     return TensorElem.nested ts
-  else 
+  else
     let n <- pnumber
     return TensorElem.int n
 
-partial def pattrvalue_dense (u: Unit): P AttrVal := do
+partial def pattrvalue_dense (u: Unit): P (AttrValue δ) := do
   pident? "dense"
   pconsume '<'
   let v <- ptensorelem ()
   pconsume '>'
   pconsume ':'
   let ty <- ptype_vector
-  return AttrVal.dense v ty   
+  return builtin.denseWithType v ty
 
 
-partial def pattrvalue_list (u: Unit): P AttrVal := do 
+partial def pattrvalue_list (u: Unit): P (AttrValue δ) := do
   let ts <- pintercalated '[' (pattrvalue ()) ','  ']'
-  return AttrVal.list ts
+  return AttrValue.list ts
 
-partial def pattrvalue (u: Unit): P AttrVal := do
+partial def pattrvalue (u: Unit): P (AttrValue δ) := do
  pnote "hunting for attribute value"
- por pattrvalue_int $ 
- por (pmap AttrVal.str pstr) $ 
- por (pmap AttrVal.type (ptype ())) $
+ por pattrvalue_int $
+ por (pmap AttrValue.str pstr) $
+ por (pmap AttrValue.type (ptype ())) $
  por (pattrvalue_list ()) $
  (pattrvalue_dense ())
 
-partial def pattr : P AttrEntry := do
+partial def pattr : P (AttrEntry δ) := do
   eat_whitespace
   let name <- pident
   eat_whitespace
@@ -141,25 +147,25 @@ partial def pattr : P AttrEntry := do
   let value <- pattrvalue ()
   return (AttrEntry.mk name value)
 
-  
 
-partial def pop (u: Unit) : P Op := do 
+
+partial def pop (u: Unit) : P (Op δ) := do
   eat_whitespace
-  match (<- ppeek) with 
+  match (<- ppeek) with
   | some '\"' => do
     let name <- pstr
     let args <- pintercalated '(' pssaval ',' ')'
-    let bbs <- (if (<- ppeek? '[' ) 
+    let bbs <- (if (<- ppeek? '[' )
                 then pintercalated '[' pbbname ','  ']'
                 else return [])
     let hasRegion <- ppeek? '('
-    let regions <- (if hasRegion 
+    let regions <- (if hasRegion
                       then pintercalated '(' (pregion ()) ',' ')'
                       else pure [])
     -- | parse attributes
     let hasAttrs <- ppeek? '{'
     let attrs <- (if hasAttrs
-              then  pintercalated '{' pattr ',' '}' 
+              then  pintercalated '{' pattr ',' '}'
               else pure [])
     pconsume ':'
     let ty <- ptype u
@@ -168,10 +174,10 @@ partial def pop (u: Unit) : P Op := do
   | other => perror ("expected '\"' or '%' to begin operation definition. found: " ++ toString other)
 
 
-partial def popcall (u: Unit) : P BasicBlockStmt := do
+partial def popcall (u: Unit) : P (BasicBlockStmt δ) := do
    eat_whitespace
    if (<- ppeek? '%')
-   then do 
+   then do
      let val <- pssaval
      pconsume '='
      let op <- pop u
@@ -182,14 +188,14 @@ partial def popcall (u: Unit) : P BasicBlockStmt := do
      return (BasicBlockStmt.StmtOp op)
 
 -- | parse a sequence of ops, with no label
-partial def pentryblock_no_label (u: Unit) : P BasicBlock := do
+partial def pentryblock_no_label (u: Unit) : P (BasicBlock δ) := do
    let ops <- pmany1 (popcall u)
    pnote $ "pentry ops: " ++ List.toString ops
    return (BasicBlock.mk "entry" [] ops)
 
 
-   
-partial def pblock (u: Unit) : P BasicBlock := do
+
+partial def pblock (u: Unit) : P (BasicBlock δ) := do
    pconsume '^'
    let name <- pident
    let args <-  (if (<- ppeek? '(')
@@ -202,7 +208,9 @@ partial def pblock (u: Unit) : P BasicBlock := do
 
 end   -- end the mutual block
 
-theorem parse_of_print_id: 
-  ∀ (o: Op), ((pop ()).runP locbegin [] (Pretty.doc o)).snd.snd.snd = Result.ok o := sorry
+theorem parse_of_print_id:
+  ∀ (o: Op δ), ((pop ()).runP locbegin [] (Pretty.doc o)).snd.snd.snd = Result.ok o := sorry
+
+end   -- end of the section defining δ
 
 end MLIR.MLIRParser
