git/opencompl/lean-mlir/MLIR/Semantics/Types.lean
@@ -1,52 +1,231 @@
 /-
 ## MLIR types
 
-This file implements support for builtin MLIR types, as well as conversion to
-concrete Lean types and values.
+This file implements general properties of MLIR types, including decidable
+equality of both types and values, Inhabited instances, and concretization of
+MLIR types to standard Lean types.
 
-In order to support the untyped SSA environment (which doesn't require name
-definitions/uses to match as this is proven later), every concrete MLIR type
-should be Inhabited so that `SSAEnvE.Get` can pretend to return default values.
+Only the types explicitly laid out in MLIRType are considered here; non-trivial
+types like tensors and user-defined types provide similar properties through
+the generic type interface.
+
+We require every concrete MLIR type to be Inhabited so that we can keep the
+`SSAEnv` untyped and have `SSAEnvE.Get` return default values in case of a
+dynamic type mismatch (which is provably impossible but extremely impractical
+to use as a guarantee).
 
 Current properly-supported MLIR built-in types:
 
-* Function type [τ₁ → τ₂]: Lean function
 * Tuple type [(τ₁, ..., τₙ)]: n-ary product of underlying types
-* Tensors [tensor<DxDx?xDx?xτ>]: RankedTensor type
+* Index type: infinite precision Int
+* Generic type: via type interface
 
 Types that need improvements or refinements:
 
+* Function type [τ₁ → τ₂]
+  Resolves to program symbols, lacks testing
+* Integer types [i32, etc]
+  TODO: Model i32/etc with finite precision, probably restarting from Fin
 * Unsigned finite integer types [u32, etc]
   TODO: Model u32/etc with lean's Uint{8/16/32/64} or restart with Fin
-* Integer types [i32, etc]: currently use Int
-  TODO: Model i32/etc properly, probably restarting from Fin
-* Float types [f16, f32, f64, f80, f128]. todo
-  No idea how to model floats of different precisions in Lean?
-* Vectors: could expand on tensors. todo
-* Unranked tensors: todo
-* User types: should use a typeclass
-  TODO: Model user types
+* Float types [f16, f32, f64, f80, f128]
+  Good luck with these
 -/
 
 import MLIR.Util.Arith
 import MLIR.Util.List
 import MLIR.Semantics.Fitree
-
 import MLIR.AST
+
+import Lean
+import Lean.Elab.Term
+import Lean.Elab.Exception
+
 open MLIR.AST
+open Lean
+open Lean.Elab
+open Lean.Elab.Term
+open Lean.Parser.Term
 
-def shape_prod: List Nat → Nat :=
-  List.foldr (·*·) 1
+section
+variable {α σ ε} [δ: Dialect α σ ε]
 
-theorem shape_prod_nil: shape_prod (0::l) = 0 := by
-  induction l <;> simp [shape_prod, List.foldr]
+/-
+### Decidable equality for MLIRType
+-/
 
-instance: OfNat Dimension (n: Nat) where
-  ofNat := Dimension.Known n
+mutual
+
+def MLIRType.eq (τ₁ τ₂: MLIRType δ): Decidable (τ₁ = τ₂) := by
+  cases τ₁ <;> cases τ₂
+  <;> try (simp; exact inferInstance)
+  <;> try apply isFalse MLIRType.noConfusion
+
+  case fn.fn a₁ b₁ a₂ b₂ =>
+    match eq a₁ a₂, eq b₁ b₂ with
+    | isTrue ha, isTrue hb => exact isTrue $ by rw [ha, hb]
+    | isFalse ha, _ => exact isFalse fun h => by cases h; cases ha rfl
+    | _, isFalse hb => exact isFalse fun h => by cases h; cases hb rfl
+
+  case tuple.tuple l₁ l₂ =>
+    match eqList l₁ l₂ with
+    | isTrue h => exact isTrue $ by rw [h]
+    | isFalse h => exact isFalse fun h' => by cases h'; cases h rfl
+
+private def MLIRType.eqList (l₁ l₂: List (MLIRType δ)): Decidable (l₁ = l₂) :=
+  match l₁, l₂ with
+  | [], [] => isTrue rfl
+  | τ₁::l₁, τ₂::l₂ =>
+      match eq τ₁ τ₂, eqList l₁ l₂ with
+      | isTrue hτ, isTrue hl => isTrue $ by rw [hτ,hl]
+      | isFalse hτ, _ => isFalse fun h => by cases h; cases hτ rfl
+      | _, isFalse hl => isFalse fun h => by cases h; cases hl rfl
+  | [], _::_ => isFalse List.noConfusion
+  | _::_, [] => isFalse List.noConfusion
+end
+
+instance: DecidableEq (MLIRType δ) :=
+  MLIRType.eq
 
 
 /-
-## Shape inference on literal tensors
+### Evaluation into concrete Lean types
+-/
+
+/- MLIRType is a nested inductive type. Recursive functions on such types are
+   compiled to well-founded recursion. This prevents it from being reduced by
+   the elaborator, so instead we define it manually with the recursor.
+   See: https://leanprover.zulipchat.com/#narrow/stream/270676-lean4/topic/reduction.20of.20dependent.20return.20type/near/276044057 -/
+
+@[reducible, simp_itree]
+def MLIR.AST.MLIRType.eval (τ: MLIRType δ): Type :=
+  MLIRType.recOn τ
+    (motive_1 := fun _ => Type) -- MLIRType
+    (motive_2 := fun _ => Type) -- List MLIRType
+    -- .fn (the only functions we can materialize are symbols)
+    (fun τ₁ τ₂ eval_τ₁ eval_τ₂ => String)
+    -- .int
+    (fun bitsize => Int)
+    -- .float
+    (fun bitsize => Float)
+    -- .index
+    Nat
+    -- .tuple [Mapping motive_2 to motive_1]
+    (fun _ ih => ih)
+    -- .undefined
+    (fun name => Unit)
+    -- .generic
+    ε
+    -- [] (in .tuple)
+    Unit
+    -- (τ::l) (in .tuple)
+    (fun τ l eval_τ eval_l =>
+      match l with
+      | [] => eval_τ
+      | _  => eval_τ × eval_l)
+
+
+/-
+### Properties of evaluated types
+
+The requirements from the type interface allow us to prove that MLIR types have
+inhabitants and a decidable equality.
+-/
+
+def MLIR.AST.MLIRType.default (τ: MLIRType δ): τ.eval :=
+  match τ with
+  | .fn τ₁ τ₂ => ""
+  | .int _ => 0
+  | .float _ => 0.0
+  | .index => 0
+  | .tuple [] => ()
+  | .tuple [τ] => τ.default
+  | .tuple (τ₁::τ₂::l) => (τ₁.default, default $ .tuple (τ₂::l))
+  | .undefined name => ()
+  | .extended s => DialectTypeIntf.inhabited s
+
+instance (τ: MLIRType δ): Inhabited τ.eval where
+  default := τ.default
+
+def MLIRType.eval.eq {τ: MLIRType δ} (v₁ v₂: τ.eval): Decidable (v₁ = v₂) :=
+  match τ with
+  | .fn τ₁ τ₂ => inferInstance
+  | .int _ => inferInstance
+  | .float _ =>
+      -- FIXME: Equality of floats
+      if v₁ == v₂ then isTrue sorry else isFalse sorry
+  | .index => inferInstance
+  | .tuple [] => inferInstance
+  | .tuple [τ] => @eq τ v₁ v₂
+  | .tuple (τ₁::τ₂::τs) =>
+      let (v₁, l₁) := v₁
+      let (v₂, l₂) := v₂
+      match eq v₁ v₂, @eq (.tuple (τ₂::τs)) l₁ l₂ with
+      | isTrue h₁, isTrue h₂ => isTrue $ by rw [h₁,h₂]
+      | isFalse h₁, _ => isFalse fun h => by cases h; cases h₁ rfl
+      | _, isFalse h₂ => isFalse fun h => by cases h; cases h₂ rfl
+  | .undefined _ => inferInstance
+  | .extended s => DialectTypeIntf.eq s v₁ v₂
+
+instance {τ: MLIRType δ}: DecidableEq τ.eval :=
+  MLIRType.eval.eq
+
+def MLIRType.eval.str {τ: MLIRType δ} (v: τ.eval): String :=
+  match τ, v with
+  | .fn τ₁ τ₂, v => v
+  | .int _, v => toString v
+  | .float _, v => toString v
+  | .index, v => toString v
+  | .tuple [], v => "()"
+  | .tuple [τ], v => "(" ++ (@str τ v).drop 1
+  | .tuple (τ₁::τ₂::τs), (v,vs) =>
+    "(" ++ str v ++ (@str (.tuple (τ₂::τs)) vs).drop 1
+  | .undefined _, () => "<undefined>"
+  | .extended s, v => DialectTypeIntf.str s v
+
+instance {τ: MLIRType δ}: ToString τ.eval where
+  toString := MLIRType.eval.str
+
+end -- of section defining δ
+
+
+/-
+## Decidable equality for TensorElem
+-/
+
+mutual
+def TensorElem.eq (e₁ e₂: TensorElem): Decidable (e₁ = e₂) := by
+  cases e₁ <;> cases e₂
+  <;> try (simp; exact inferInstance)
+  <;> try apply isFalse TensorElem.noConfusion
+
+  case float.float f₁ f₂ =>
+    -- FIXME: We shouldn't have DecidableEq on floats o(x_x)o
+    exact if f₁ == f₂ then isTrue sorry else isFalse sorry
+
+  case nested.nested l₁ l₂ =>
+    match eqList l₁ l₂ with
+    | isTrue h => exact isTrue $ by rw [h]
+    | isFalse h => exact isFalse fun h' => by cases h'; cases h rfl
+
+private def TensorElem.eqList (l₁ l₂: List TensorElem): Decidable (l₁ = l₂) :=
+  match l₁, l₂ with
+  | [], [] => isTrue rfl
+  | e₁::l₁, e₂::l₂ =>
+      match eq e₁ e₂, eqList l₁ l₂ with
+      | isTrue hτ, isTrue hl => isTrue $ by rw [hτ,hl]
+      | isFalse hτ, _ => isFalse fun h => by cases h; cases hτ rfl
+      | _, isFalse hl => isFalse fun h => by cases h; cases hl rfl
+  | [], _::_ => isFalse List.noConfusion
+  | _::_, [] => isFalse List.noConfusion
+end
+
+instance: DecidableEq TensorElem :=
+  TensorElem.eq
+
+
+/-
+## Shape inference on TensorElem
 
 This section defines shape verification and shape inference for TensorElem
 (tensor literals), *excluding the case of uniform tensor literals*. The shape
@@ -58,6 +237,12 @@ ranked tensors and properly handle uniform tensor literals.
 
 TODO: Integrate TensorElem invariants into the verifier
 -/
+
+def shape_prod: List Nat → Nat :=
+  List.foldr (·*·) 1
+
+theorem shape_prod_nil: shape_prod (0::l) = 0 := by
+  induction l <;> simp [shape_prod, List.foldr]
 
 namespace MLIR.AST.TensorElem
 
@@ -83,13 +268,13 @@ def hasShape: TensorElem → List Nat → Bool
       false
 
 -- Check whether a tensor literal has a particular data type
-def hasType: TensorElem → MLIRTy → Bool
-  | TensorElem.int _, MLIRTy.int _ =>
+def hasType: TensorElem → MLIRType δ → Bool
+  | TensorElem.int _, .int _ =>
       -- TODO: Check bounds
       true
-  | TensorElem.bool _, MLIRTy.int 1 =>
+  | TensorElem.bool _, .int 1 =>
       true
-  | TensorElem.float _, MLIRTy.float _ =>
+  | TensorElem.float _, .float _ =>
       true
   | TensorElem.nested [], τ =>
       true
@@ -98,21 +283,25 @@ def hasType: TensorElem → MLIRTy → Bool
   | _, _ =>
       false
 
-def hasType_list_1 {l τ}: hasType (.nested l) τ → l.all (hasType . τ) := by
+def hasType_list_1 {l} {τ: MLIRType δ}:
+    hasType (.nested l) τ → l.all (hasType . τ) := by
   induction l; simp
   case cons e l ih =>
     simp [hasType, List.all_cons]
     intro h
-    simp [ih h.2, h.1]
+    simp [h.1]
+    apply ih h.2
 
-def hasType_list_2 {l τ}: l.all (hasType . τ) → hasType (.nested l) τ := by
+def hasType_list_2 {l} {τ: MLIRType δ}:
+    l.all (hasType . τ) → hasType (.nested l) τ := by
   induction l; simp [hasType]
   case cons e l ih =>
     simp [hasType, List.all_cons]
     intro h
-    simp [ih h.2, h.1]
+    simp [h.1]
+    apply ih h.2
 
-def mapWithType {α τ} l (f: (e: TensorElem) → (h: e.hasType τ) → α)
+def mapWithType {α} {τ: MLIRType δ} l (f: (e: TensorElem) → (h: e.hasType τ) → α)
     (h: hasType (TensorElem.nested l) τ): List α :=
   match l, h with
   | [], h =>
@@ -247,13 +436,7 @@ end MLIR.AST.TensorElem
 
 
 /-
-### Vector types
-TODO: Not modeled fully by lean-mlir right now
--/
-
-
-/-
-### Ranked tensors
+### Tools for generation of ranked tensors
 TODO: Consider a different type KnownRankedTensor that we could project to if
 TODO| we have known dimensions. Everything is conditioned by DimList.known...
 -/
@@ -268,6 +451,8 @@ def shape_refines: List Nat → List Dimension → Bool
 
 @[inline]
 def DimList := List Dimension
+
+deriving instance DecidableEq for DimList
 
 @[simp]
 def DimList.prod: DimList → Nat
@@ -338,218 +523,19 @@ theorem default_refinement_refines (D: DimList):
   case cons head _ ih =>
     cases head <;> simp <;> apply ih
 
--- Ranked tensors have known rank but possibly unknown dimensions. At runtime,
--- the size is fully determined. We store the visible type information in the
--- parameters of RankedTensor, and collect the fully-specified runtime data in
--- the structure fields.
---
--- We add an intermediate [size] parameter so that we can separate data
--- manipulation and proofs about the product of the dimensions, which would
--- otherwise be tricky due to [Fin] constantly carrying proofs.
-structure RankedTensor (α: Type) (D: DimList) where
-  -- Actual dimensions
-  shape: List Nat
-  -- Contents; we use a function for brevity
-  -- TODO: RankedTensor: Consider a more computable data storage method
-  data: List α
-  -- Invariants: shape/dimension must be compatible, shape/size must match
-  h_refines: shape_refines shape D
-  h_data_size: data.length = shape_prod shape
-
-theorem RankedTensor.eq_of_fields_eq (α D): ∀ (t₁ t₂: RankedTensor α D),
-  t₁.shape = t₂.shape →
-  t₁.data = t₂.data →
-    t₁ = t₂ := by
-  intros t₁ t₂ Hshape Hdata
-  cases t₁; cases t₂; simp at *
-  trivial
-
-def RankedTensor.uniform {α} D (v: α): RankedTensor α D :=
-  { shape       := D.default_refinement,
-    data        := List.uniform v (shape_prod D.default_refinement),
-    h_refines   := default_refinement_refines _,
-    h_data_size := List.uniform_length _ _ }
-
-def RankedTensor.default α D [Inhabited α]: RankedTensor α D :=
-  RankedTensor.uniform D Inhabited.default
-
-instance {α D} [Inhabited α]: Inhabited (RankedTensor α D) where
-  default := RankedTensor.default α D
-
-
-/-
-### Unranked tensors
-TODO: Unranked tensors?
--/
-
-
-/-
-### Evaluation of MLIR types
-TODO: Not all MLIRTy types are correctly evaluated
--/
-
-/- MLIRTy is a nested inductive type, thus defined with well-founded recursion.
-   This prevents it from being reduced by the elaborator, so instead we define
-   it manually with the recursor.
-   See: https://leanprover.zulipchat.com/#narrow/stream/270676-lean4/topic/
-   reduction.20of.20dependent.20return.20type/near/276044057 -/
-
-@[reducible, simp_itree]
-def MLIR.AST.MLIRTy.eval (τ: MLIRTy): Type :=
-  @MLIRTy.rec
-    (motive_1  := fun _ => Type) -- MemrefLayoutSpec
-    (motive_2  := fun _ => Type) -- MLIRTy
-    (motive_3  := fun _ => Type) -- AttrVal
-    (motive_4  := fun _ => Type) -- AttrEntry
-    (motive_5  := fun _ => Type) -- AttrDict
-    (motive_6  := fun _ => Type) -- List MLIRTy
-    (motive_7  := fun _ => Type) -- Option MemrefLayoutSpec
-    (motive_8  := fun _ => Type) -- Option AttrVal
-    (motive_9  := fun _ => Type) -- List AttrVal
-    (motive_10 := fun _ => Type) -- List AttrEntry
-
-    -- **MemrefLayoutSpec**
-
-    -- MemrefLayoutSpec.stride
-    (fun offset stride => Unit)
-    -- MemrefLayoutSpec.attr (this is the one which loops everything)
-    (fun attr eval_attr => Unit)
-
-    -- **MLIRTy**
-
-    -- MLIRTy.fn
-    (fun τ₁ τ₂ eval_τ₁ eval_τ₂ => eval_τ₁ → eval_τ₂)
-    -- MLIRTy.int
-    (fun bitsize => Int)
-    -- MLIRTy.float
-    (fun bitsize => Float)
-    -- MLIRTy.index
-    Nat
-    -- MLIRTy.tuple [Mapping motive_2 to motive_1]
-    (fun _ ih => ih)
-    -- MLIRTy.vector (todo)
-    (fun Dfixed Dscaled τ eval_τ => Unit)
-    -- MLIRTy.tensorRanked (todo)
-    (fun D τ eval_τ => RankedTensor eval_τ D)
-    -- MLIRTy.tensorUnranked (todo)
-    (fun τ eval_τ => Unit)
-    -- MLIRTy.memrefRanked (todo)
-    (fun D τ eval_τ layout eval_layout memspace eval_memspace => Unit)
-    -- MLIRTy.memrefUnranked (todo)
-    (fun τ eval_τ memspace eval_memspace => Unit)
-    -- MLIRTy.user (todo)
-    (fun name => Unit)
-
-    -- **AttrVal**
-
-    -- AttrVal.symbol
-    (fun symbol => Unit)
-    -- AttrVal.str
-    (fun str => Unit)
-    -- AttrVal.int
-    (fun int τ eval_τ => Unit)
-    -- AttrVal.bool
-    (fun bool => Unit)
-    -- AttrVal.float
-    (fun float τ eval_τ => Unit)
-    -- AttrVal.type
-    (fun τ eval_τ => Unit)
-    -- AttrVal.dense
-    (fun el τ eval_τ => Unit)
-    -- AttrVal.affine
-    (fun affine_map => Unit)
-    -- AttrVal.list
-    (fun list eval_list => Unit)
-    -- AttrVal.nestedsymbol
-    (fun a₁ eval_a₁ a₂ eval_a₂ => Unit)
-    -- AttrVal.alias
-    (fun str => Unit)
-    -- AttrVal.dict
-    (fun dict eval_dict => Unit)
-    -- AttrVal.opaque
-    (fun dialect value => Unit)
-    -- AttrVal.opaqueElements
-    (fun dialect value τ eval_τ => Unit)
-    -- AttrVal.unit
-    Unit
-
-    -- **AttrEntry**
-
-    -- AttrEntry.mk
-    (fun key value eval_value => Unit)
-
-    -- **AttrDict**
-
-    -- AttrDict.mk
-    (fun list eval_list => Unit)
-
-    -- **List MLIRTy** (in MLIRTy.tuple)
-
-    -- []
-    Unit
-    -- (τ::l)
-    (fun τ l eval_τ eval_l =>
-      match l with
-      | [] => eval_τ
-      | _  => eval_τ × eval_l)
-
-    -- **Option MemrefLayoutSpec**
-
-    Unit
-    (fun layout eval_layout => Unit)
-
-    -- **Option AttrVal**
-
-    Unit
-    (fun attr eval_attr => Unit)
-
-    -- **List AttrVal**
-
-    Unit
-    (fun head tail eval_head eval_tail => Unit)
-
-    -- **List AttrEntry**
-
-    Unit
-    (fun head tail eval_head eval_tail => Unit)
-
-  -- The subject of the induction
-  τ
-
-def MLIR.AST.MLIRTy.default (τ: MLIRTy): τ.eval :=
-  match τ with
-  | MLIRTy.fn τ₁ τ₂ => (fun _ => τ₂.default)
-  | MLIRTy.int _ => 0
-  | MLIRTy.float _ => 0.0
-  | MLIRTy.index => 0
-  | MLIRTy.tuple [] => ()
-  | MLIRTy.tuple [τ] => τ.default
-  | MLIRTy.tuple (τ₁::τ₂::l) => (τ₁.default, (MLIRTy.tuple (τ₂::l)).default)
-  | MLIRTy.vector _ _ _ => () /- todo -/
-  | MLIRTy.tensorRanked D τ => @RankedTensor.default τ.eval D ⟨default τ⟩
-  | MLIRTy.tensorUnranked τ => () /- todo -/
-  | MLIRTy.memrefRanked D τ _ _ => () /- todo -/
-  | MLIRTy.memrefUnranked τ _ => () /- todo -/
-  | MLIRTy.user _ => () /- todo -/
-
-instance (τ: MLIRTy): Inhabited τ.eval where
-  default := τ.default
-
-
----
-
--- TODO: RankedTensor.ofTensorElem: account for typing?
--- Which allows us to flatten the term into a single array for a RankedTensor
 
 namespace MLIR.AST.TensorElem
 
-def flatten {τ} (e: TensorElem) (h: e.hasType τ): List τ.eval :=
+section
+variable {α σ ε} {δ: Dialect α σ ε}
+
+def flatten {τ: MLIRType δ} (e: TensorElem) (h: e.hasType τ): List τ.eval :=
   match e, τ with
-  | TensorElem.int i, MLIRTy.int _ =>
+  | TensorElem.int i, .int _ =>
       [i]
-  | TensorElem.bool b, MLIRTy.int _ =>
+  | TensorElem.bool b, .int _ =>
       [if b then 1 else 0]
-  | TensorElem.float f, MLIRTy.float _ =>
+  | TensorElem.float f, .float _ =>
       [f]
   | TensorElem.nested [], _ =>
       []
@@ -562,7 +548,7 @@ def flatten {τ} (e: TensorElem) (h: e.hasType τ): List τ.eval :=
 
 -- Once again, we prove a more friendly version of the list case first
 
-theorem flatten_list {τ} (l: List TensorElem) (h: hasType (.nested l) τ):
+theorem flatten_list {τ: MLIRType δ} (l: List TensorElem) (h: hasType (.nested l) τ):
     flatten (.nested l) h = (mapWithType l flatten h).join := by
   revert h
   induction l <;> intros h
@@ -571,7 +557,7 @@ theorem flatten_list {τ} (l: List TensorElem) (h: hasType (.nested l) τ):
   case cons _ _ ih =>
     simp [flatten, mapWithType, List.join, ih]
 
-theorem flatten_size {τ} (e: TensorElem) (shape: List Nat):
+theorem flatten_size {τ: MLIRType δ} (e: TensorElem) (shape: List Nat):
     e.hasShape shape → (h: e.hasType τ) → (e.flatten h).length = shape_prod shape := by
   revert shape
   apply @TensorElem.recOn
@@ -616,37 +602,22 @@ theorem flatten_size {τ} (e: TensorElem) (shape: List Nat):
     simp [IH2 s Hshape.2 Htype.2]
     rw [motive_1 s Hshape.1 Htype.1]
 
-inductive rankCompatibleWith (e: TensorElem) (D: DimList): MLIRTy → Type :=
+inductive rankCompatibleWith (e: TensorElem) (D: DimList): MLIRType δ → Type :=
   | UniformInt (i: Int) bitsize:
       -- TODO: Check range of uniform tensor value
       e = TensorElem.int i →
-      e.rankCompatibleWith D (MLIRTy.int bitsize)
+      e.rankCompatibleWith D (.int bitsize)
   | UniformBool (b: Bool):
       e = TensorElem.bool b →
-      e.rankCompatibleWith D (MLIRTy.int 1)
+      e.rankCompatibleWith D (.int 1)
   | UniformFloat (f: Float) bitsize:
       -- TODO: Check range of uniform tensor value
       e = TensorElem.float f →
-      e.rankCompatibleWith D (MLIRTy.float bitsize)
+      e.rankCompatibleWith D (.float bitsize)
   | HasShape s τ:
       e.hasShape s →
       shape_refines s D →
       e.rankCompatibleWith D τ
 
+end
 end MLIR.AST.TensorElem
-
-def RankedTensor.ofTensorElem {τ} (D: DimList) (e: TensorElem)
-    (Htype: e.hasType τ) (Hcompat: e.rankCompatibleWith D τ):
-    RankedTensor τ.eval D:=
-  match Hcompat with
-  | .UniformInt i bitsize _ =>
-      RankedTensor.uniform D i
-  | .UniformBool b _ =>
-      RankedTensor.uniform D (if b then 1 else 0)
-  | .UniformFloat f bitsize _ =>
-      RankedTensor.uniform D f
-  | .HasShape s τ Hshape Hrefines =>
-      { shape       := s,
-        data        := e.flatten Htype,
-        h_refines   := Hrefines,
-        h_data_size := TensorElem.flatten_size e s Hshape Htype }
