git/opencompl/lean-mlir/MLIR/Dialects/BuiltinModel.lean
@@ -1,0 +1,362 @@
+/-
+# Data model for the built-in dialect
+-/
+
+import MLIR.AST
+import MLIR.Doc
+import MLIR.Semantics.Types
+open MLIR.AST
+
+/-
+## General tensor type
+
+The following structure is used as the basis for both ranked and unranked
+tensor types, since both have the same runtime contents and only differ by the
+amount of information exposed in the typing system.
+
+At runtime the dimension of tensors is always known. As a general rule, we
+store compile-time type information in the parameters of the structure and the
+runtime contents in the fields.
+-/
+
+structure Tensor (τ: MLIRTy) where
+  -- Runtime-determined dimensions
+  shape: List Nat
+  -- Contents in row-major order
+  data: List τ.eval
+  -- Invariant: shape and size must match
+  h_data_size: data.length = shape_prod shape
+
+theorem Tensor.eq_of_fields_eq {τ} (t₁ t₂: Tensor τ):
+    t₁.shape = t₂.shape → t₁.data = t₂.data → t₁ = t₂ := by
+  intros h_shape h_data
+  cases t₁; cases t₂; simp at *
+  trivial
+
+instance {τ}: DecidableEq (Tensor τ) := fun t₁ t₂ => by
+  cases t₁; cases t₂; simp
+  exact inferInstance
+
+def Tensor.uniform {τ} (shape: List Nat) (v: τ.eval): Tensor τ :=
+  { shape       := shape,
+    data        := List.uniform v (shape_prod shape),
+    h_data_size := List.length_uniform _ _ }
+
+instance {τ}: Inhabited (Tensor τ) where
+  default := Tensor.uniform [1] default
+
+
+/-
+## Ranked tensor type
+
+A ranked tensor extends the runtime tensor with a statically-known list of
+dimensions (all of which may not be known) which adds more invariants.
+-/
+
+structure RankedTensor (D: DimList) (τ: MLIRTy) extends Tensor τ where
+  -- Invariants: shape/dimension must be compatible, shape/size must match
+  h_refines: shape_refines shape D
+
+theorem RankedTensor.eq_of_fields_eq {τ D} (t₁ t₂: RankedTensor τ D):
+    t₁.shape = t₂.shape → t₁.data = t₂.data → t₁ = t₂ := by
+  intros h_shape h_data
+  suffices t₁.toTensor = t₂.toTensor by
+    cases t₁; cases t₂; simp at *; trivial
+  apply Tensor.eq_of_fields_eq <;> trivial
+
+instance {τ D}: DecidableEq (RankedTensor τ D) := fun t₁ t₂ => by
+  cases t₁; cases t₂; simp
+  exact inferInstance
+
+def RankedTensor.uniform {τ} (D: DimList) (v: τ.eval): RankedTensor D τ :=
+  { Tensor.uniform D.default_refinement v with
+    h_refines   := default_refinement_refines _ }
+
+instance {τ D}: Inhabited (RankedTensor D τ) where
+  default := RankedTensor.uniform D default
+
+def RankedTensor.typeStr (τ: MLIRTy) (D: DimList): String :=
+  let dims := "x".intercalate (D.map (MLIR.Doc.Pretty.doc ·))
+  s!"tensor<{dims}x{τ}>"
+
+-- TODO: String representation of ranked tensors
+def RankedTensor.str {τ D} (t: RankedTensor D τ): String :=
+  let dims := "×".intercalate (D.map (MLIR.Doc.Pretty.doc ·))
+  s!"<a tensor of size {dims} and base type {τ}>"
+
+-- Conversion from TensorElem
+
+def RankedTensor.ofTensorElem {τ} (D: DimList) (e: TensorElem)
+    (Htype: e.hasType τ) (Hcompat: e.rankCompatibleWith D τ):
+    RankedTensor D τ :=
+  match Hcompat with
+  | .UniformInt i bitsize _ =>
+      RankedTensor.uniform D i
+  | .UniformBool b _ =>
+      RankedTensor.uniform D (if b then 1 else 0)
+  | .UniformFloat f bitsize _ =>
+      RankedTensor.uniform D f
+  | .HasShape s τ Hshape Hrefines =>
+      { shape       := s,
+        data        := e.flatten Htype,
+        h_refines   := Hrefines,
+        h_data_size := TensorElem.flatten_size e s Hshape Htype }
+
+-- Type interface for registration with MLIRType
+
+private abbrev σ_RankedTensor := DimList × MLIRTy
+private abbrev ε_RankedTensor := fun (D, τ) => RankedTensor D τ
+
+instance: DialectTypeIntf σ_RankedTensor ε_RankedTensor where
+  inhabited := default
+  typeEq := inferInstance
+  eq := inferInstance
+  str := fun (τ, D) t => t.str
+  typeStr := fun (τ, D) => RankedTensor.typeStr D τ
+
+
+/-
+## Unranked tensor type
+-/
+
+abbrev UnrankedTensor := Tensor
+
+-- Type interface for registration with MLIRType
+
+private abbrev σ_UnrankedTensor := MLIRTy
+private abbrev ε_UnrankedTensor := UnrankedTensor
+
+def UnrankedTensor.typeStr (τ: MLIRTy): String :=
+  s!"tensor<*{τ}>"
+
+-- TODO: String representation of ranked tensors
+def UnrankedTensor.str {τ} (t: UnrankedTensor τ) :=
+  s!"<an unranked tensor of base type {τ}>"
+
+instance: DialectTypeIntf σ_UnrankedTensor ε_UnrankedTensor where
+  inhabited := default
+  typeEq := inferInstance
+  eq := inferInstance
+  str := @UnrankedTensor.str
+  typeStr := UnrankedTensor.typeStr
+
+
+/-
+## Vector type
+-/
+
+def Vector.size (fixed scalable: List Nat) (scale: List Nat)
+    (H: scale.length = scalable.length) :=
+  shape_prod fixed * shape_prod (List.map₂ (· * ·) scalable scale)
+
+structure Vector (fixed: List Nat) (scalable: List Nat) (τ: MLIRTy) where
+  -- Scales (number of instantiations of each scalable dimension)
+  scale: List Nat
+  -- Contents in row-major order
+  data: List τ.eval
+  -- Invariant: Number of scales must match number of scalable dimensions
+  h_scale_size: scale.length = scalable.length
+  -- Invariant: Number of data elements must match scale
+  h_data_size: data.length = Vector.size fixed scalable scale h_scale_size
+
+theorem Vector.eq_of_fields_eq (v₁ v₂: Vector τ fixed scalable):
+    v₁.scale = v₂.scale → v₁.data = v₂.data → v₁ = v₂ := by
+  intros h_scale h_data
+  cases v₁; cases v₂; simp at *
+  trivial
+
+instance: Inhabited (Vector fixed scalable τ) where
+  default :=
+    { scale := List.map (fun _ => 1) scalable,
+      data := List.uniform default (Vector.size fixed scalable
+                (List.map (fun _ => 1) scalable) (by apply List.length_map)),
+      h_scale_size := by apply List.length_map,
+      h_data_size := by apply List.length_uniform }
+
+instance: DecidableEq (Vector τ fixed scalable) := fun v₁ v₂ =>
+  if h: v₁.scale = v₂.scale ∧ v₁.data = v₂.data then
+    isTrue (by apply Vector.eq_of_fields_eq _ _ h.1 h.2)
+  else
+    isFalse fun h' => by simp [h'] at *
+
+def Vector.typeStr (fixed scalable: List Nat) (τ: MLIRTy) :=
+  let sf := "x".intercalate (fixed.map (MLIR.Doc.Pretty.doc ·))
+  let ss := "x".intercalate (scalable.map (MLIR.Doc.Pretty.doc ·))
+
+  if fixed.length > 0 && scalable.length > 0 then
+    s!"vector<{sf}x[{ss}]x{τ}>"
+  else if fixed.length > 0 then
+    s!"vector<{sf}x{τ}>"
+  else if scalable.length > 0 then
+    s!"vector<[{ss}]x{τ}>"
+  else
+    s!"vector<{τ}>"
+
+-- TODO: String representation of vector values
+def Vector.str (v: Vector fixed scalable τ): String :=
+  let str_type := Vector.typeStr fixed scalable τ
+  s!"<a vector of type {str_type}>"
+
+-- Type interface for registration with MLIRType
+
+private abbrev σ_Vector := List Nat × List Nat × MLIRTy
+private abbrev ε_Vector := fun (fixed, scalable, τ) => Vector fixed scalable τ
+
+instance: DialectTypeIntf σ_Vector ε_Vector where
+  inhabited := default
+  typeEq := inferInstance
+  eq := inferInstance
+  str := fun (τ, fixed, scalable) t => t.str
+  typeStr := fun (τ, fixed, scalable) => Vector.typeStr τ fixed scalable
+
+
+/-
+## TODO: Memref types
+-/
+
+inductive MemrefLayoutSpec where
+| stride: (offset: Dimension) -> (stride: List Dimension) -> MemrefLayoutSpec
+| attr: AttrVal -> MemrefLayoutSpec
+
+partial def docMemrefLayoutSpec(spec: MemrefLayoutSpec) : MLIR.Doc.Doc :=
+match spec with
+| MemrefLayoutSpec.stride offset strides => [doc| "offset:" offset ", strides: " "[" (strides),* "]"]
+| MemrefLayoutSpec.attr v => docAttrVal v
+
+-- Text representation
+/-| MLIRTy.memrefRanked dims ty layout? memspace? =>
+    let docLayout := match layout? with | some x => [doc| "," (docMemrefLayoutSpec x)] | none => ""
+    let docMemspace := match memspace? with | some x => [doc| "," (docAttrVal x)] | none => ""
+    [doc| "memref<" (intercalate_doc dims "x") "x" (go ty) (docLayout)  (docMemspace) ">"]
+  | MLIRTy.memrefUnranked ty memspace? =>
+    let docMemspace := match memspace? with | some x => [doc| "," (docAttrVal x)] | none => ""
+    [doc| "memref<" "*x" (go ty) (docMemspace) ">"] -/
+
+
+/-
+## Summary of types
+-/
+
+abbrev builtin.σ :=
+  (σ_RankedTensor ⊕ σ_UnrankedTensor) ⊕ σ_Vector
+abbrev builtin.ε :=
+  Sum.cases
+    (Sum.cases ε_RankedTensor ε_UnrankedTensor)
+    ε_Vector
+
+@[matchPattern]
+def builtin.σ.tensor (D: DimList) (τ: MLIRTy): builtin.σ :=
+  Sum.inl (Sum.inl (D, τ))
+
+@[matchPattern]
+def builtin.σ.tensor_unranked (τ: MLIRTy): builtin.σ :=
+  Sum.inl (Sum.inr τ)
+
+@[matchPattern]
+def builtin.σ.vector (fixed scalable: List Nat) (τ: MLIRTy): builtin.σ :=
+  Sum.inr (fixed, scalable, τ)
+
+
+/-
+## Dense vector/tensor attribute
+-/
+
+structure DenseAttr: Type where
+  elem: TensorElem
+  τ_sig: builtin.σ
+deriving DecidableEq
+
+-- TODO: String representation of dense<> attributes via TensorElem
+def DenseAttr.str (a: DenseAttr): String :=
+  let τ_str :=
+    match a.τ_sig with
+    | builtin.σ.tensor τ D => RankedTensor.typeStr D τ
+    | builtin.σ.tensor_unranked τ => UnrankedTensor.typeStr τ
+    | builtin.σ.vector f s τ => Vector.typeStr f s τ
+  s!"dense<...>: {τ_str}"
+
+private abbrev α_DenseAttr := DenseAttr
+
+instance: DialectAttrIntf α_DenseAttr where
+  eq := inferInstance
+  str := DenseAttr.str
+
+
+/-
+## Summary of attributes
+-/
+
+abbrev builtin.α :=
+  α_DenseAttr
+
+
+/-
+## Builtin dialect definition
+-/
+
+instance builtin: Dialect builtin.α builtin.σ builtin.ε where
+  iα := inferInstance
+  iε := inferInstance
+
+-- Custom types
+
+@[matchPattern]
+def builtin.tensor (D: DimList) (τ: MLIRTy): MLIRType builtin :=
+  MLIRType.extended (builtin.σ.tensor D τ)
+
+@[matchPattern]
+def builtin.tensor_unranked (τ: MLIRTy): MLIRType builtin :=
+  MLIRType.extended (builtin.σ.tensor_unranked τ)
+
+@[matchPattern]
+def builtin.vector (fixed scalable: List Nat) (τ: MLIRTy):
+    MLIRType builtin :=
+  MLIRType.extended (builtin.σ.vector fixed scalable τ)
+
+@[matchPattern]
+def builtin.memref (D: DimList) (τ: MLIRTy) (layout: Option MemrefLayoutSpec)
+    (memspace: Option AttrVal): MLIRType builtin :=
+  MLIRType.undefined "builtin.memref"
+
+@[matchPattern]
+def builtin.memref_unranked (τ: MLIRTy) (memspace: Option AttrVal):
+    MLIRType builtin :=
+  MLIRType.undefined "builtin.memref_unranked"
+
+-- Custom attributes
+
+@[matchPattern]
+def builtin.dense_vector_attr (e: TensorElem) (fixed scalable: List Nat)
+    (τ: MLIRTy): AttrValue builtin :=
+  AttrValue.extended (DenseAttr.mk e (builtin.σ.vector fixed scalable τ))
+
+@[matchPattern]
+def builtin.dense_tensor_attr (e: TensorElem) (D: DimList) (τ: MLIRTy):
+    AttrValue builtin :=
+  AttrValue.extended (DenseAttr.mk e (builtin.σ.tensor D τ))
+
+@[matchPattern]
+def builtin.dense_attr (e: TensorElem) {s: builtin.σ}: AttrValue builtin :=
+  AttrValue.extended (DenseAttr.mk e s)
+
+
+/-
+## High-level utilities
+-/
+
+-- Create a dense vector from a vector type
+-- FIXME: Does AttrVal.dense actually also support tensor types??
+def builtin.denseWithType (e: TensorElem) (τ: MLIRType builtin):
+    AttrValue builtin :=
+  match τ with
+  | builtin.tensor D τ =>
+      builtin.dense_tensor_attr e D τ
+  | builtin.vector fixed scalable τ =>
+      builtin.dense_vector_attr e fixed scalable τ
+  | _ =>
+      panic s!"buitin.denseVectorWithType: {τ} not a vector type"
+
+-- Create a dense vector with values `xs` and type `vector<len(xs)*ity>`
+def builtin.denseVectorOfList (xs: List Int) (ity: MLIRTy := .int 32):
+    AttrValue builtin :=
+  builtin.dense_vector_attr xs [xs.length] [] ity
