git/opencompl/lean-mlir/MLIR/Dialects/ToySemantics.lean
@@ -1,9 +1,11 @@
 import MLIR.Dialects.ToyModel
+import MLIR.Dialects.BuiltinModel
 import MLIR.Semantics.Fitree
 import MLIR.Semantics.Verifier
 import MLIR.Semantics.SSAEnv
 import MLIR.Semantics.InvalidOp
 import MLIR.Util.Metagen
+import MLIR.Util.Reduce
 
 import MLIR.AST
 import MLIR.EDSL
@@ -15,48 +17,46 @@ open MLIR.AST
 
 /- To be automatically generated -/
 
-set_option hygiene false in
-genInductive ToyOp #[
-  OpSpec.mk "Constant" `(
-    (D: DimList) → (Hknown: D.known) →
-    (e: TensorElem) → (τ: MLIRTy) → (Htype: e.hasType τ) →
-    (Hcompat: e.rankCompatibleWith D τ) →
-    ToyOp (RankedTensor τ.eval D)),
-  OpSpec.mk "Transpose" `(
-    (α: Type) → (n m: Nat) →
-    RankedTensor α [Dimension.Known n, Dimension.Known m] →
-    ToyOp (RankedTensor α [Dimension.Known m, Dimension.Known n])),
-  OpSpec.mk "Reshape" `(
-    (α: Type) → (D D': DimList) → (H: D.known) → (H': D'.known) →
-    (Hprod: D'.prod = D.prod) →
-    RankedTensor α D →
-    ToyOp (RankedTensor α D'))
-]
+inductive ToyOp: Type → Type :=
+  | Constant:
+      (D: DimList) → (Hknown: D.known) →
+      (e: TensorElem) → (τ: MLIRTy) → (Htype: e.hasType τ) →
+      (Hcompat: e.rankCompatibleWith D τ) →
+      ToyOp (RankedTensor D τ)
+  | Transpose:
+      (τ: MLIRTy) → (n m: Nat) →
+      RankedTensor [Dimension.Known n, Dimension.Known m] τ →
+      ToyOp (RankedTensor [Dimension.Known m, Dimension.Known n] τ)
+  | Reshape:
+      (τ: MLIRTy) → (D D': DimList) → (H: D.known) → (H': D'.known) →
+      (Hprod: D'.prod = D.prod) →
+      RankedTensor D τ →
+      ToyOp (RankedTensor D' τ)
 
 /- To be automatically generated (hopefully; basically this is the
    verification stuff) -/
 
 def toy_semantics_op (ret_name: Option SSAVal):
-      Op → Fitree (InvalidOpE +' SSAEnvE +' ToyOp) Unit
+      Op builtin → Fitree (InvalidOpE +' SSAEnvE builtin +' ToyOp) Unit
 
   | Op.mk "toy.constant" [] [] [] attrs
-        (MLIRTy.fn (MLIRTy.tuple []) (MLIRTy.tensorRanked D₁ τ₁)) =>
+        (.fn (.tuple []) (builtin.tensor D₁ τ₁)) =>
       match AttrDict.find attrs "value" with
-      | some (AttrVal.dense elem (MLIRTy.tensorRanked D₂ τ₂)) =>
+      | some (builtin.dense_tensor_attr elem D₂ τ₂) =>
           if H: D₁ = D₂ ∧ DimList.known D₁ ∧ τ₁ = τ₂ ∧ elem.hasType τ₁ then
             match Heq: elem, τ₁ with
-            | TensorElem.int i, MLIRTy.int 32 => do
+            | TensorElem.int i, .int 32 => do
                 let t ← Fitree.trigger (ToyOp.Constant D₁ H.2.1 elem
-                  (MLIRTy.int 32) (by simp [Heq, H.2.2.2])
+                  (.int 32) (by simp [Heq, H.2.2.2])
                   (TensorElem.rankCompatibleWith.UniformInt i 32 Heq));
-                SSAEnv.set? (MLIRTy.tensorRanked D₁ (MLIRTy.int 32)) ret_name t
+                SSAEnv.set? (builtin.tensor D₁ (.int 32)) ret_name t
             | elem, τ₁ => do
                 if Hshape: elem.hasShape (DimList.default_refinement D₁) then
                   let t ← Fitree.trigger (ToyOp.Constant D₁ H.2.1 elem τ₁
                     H.2.2.2 (TensorElem.rankCompatibleWith.HasShape
-                     (DimList.default_refinement D₁) _ Hshape
-                     (default_refinement_refines D₁)));
-                  SSAEnv.set? (MLIRTy.tensorRanked D₁ τ₁) ret_name t
+                    (DimList.default_refinement D₁) _ Hshape
+                    (default_refinement_refines D₁)));
+                  SSAEnv.set? (builtin.tensor D₁ τ₁) ret_name t
                 else
                   Fitree.trigger InvalidOpE.InvalidOp
           else
@@ -64,41 +64,37 @@ def toy_semantics_op (ret_name: Option SSAVal):
       | _ =>
           Fitree.trigger InvalidOpE.InvalidOp
 
-  | Op.mk "toy.transpose" [t_name] [] [] _ (MLIRTy.fn τ₁ τ₂) =>
-      match τ₁ with
-      | MLIRTy.tensorRanked [Dimension.Known n, Dimension.Known m] τ => do
-          let t ← Fitree.trigger (@SSAEnvE.Get (MLIRTy.tensorRanked
-                  [Dimension.Known n, Dimension.Known m] τ) _ t_name);
-          let t' ← Fitree.trigger (ToyOp.Transpose τ.eval n m t);
-          SSAEnv.set? (MLIRTy.tensorRanked [Dimension.Known m,
-                       Dimension.Known n] τ)
+  | Op.mk "toy.transpose" [t_name] [] [] _ (.fn (builtin.tensor D τ) τ₂) =>
+      match D with
+      | [Dimension.Known n, Dimension.Known m] => do
+          let t ← Fitree.trigger (SSAEnvE.Get (builtin.tensor
+                  [Dimension.Known n, Dimension.Known m] τ) t_name);
+          let t' ← Fitree.trigger (ToyOp.Transpose τ n m t);
+          SSAEnv.set? (builtin.tensor [Dimension.Known m, Dimension.Known n] τ)
             ret_name t'
       | _ =>
           Fitree.trigger InvalidOpE.InvalidOp
 
-  | Op.mk "toy.reshape" [t_name] [] [] _ (MLIRTy.fn τ₁ τ₂) =>
-      match τ₁, τ₂ with
-      | MLIRTy.tensorRanked D σ₁, MLIRTy.tensorRanked D' σ₂ =>
-          if H: σ₁ = σ₂
-             ∧ DimList.known D
-             ∧ DimList.known D'
-             ∧ DimList.prod D' = DimList.prod D then do
-            let t ← Fitree.trigger (@SSAEnvE.Get (MLIRTy.tensorRanked D σ₁) _
-                    t_name);
-            let t' ← Fitree.trigger (ToyOp.Reshape σ₁.eval D D'
-                     H.2.1 H.2.2.1 H.2.2.2 t);
-            let t': RankedTensor σ₂.eval D' := cast (by rw [H.1]) t';
-            SSAEnv.set? (MLIRTy.tensorRanked D' σ₂) ret_name t'
-          else
-            Fitree.trigger InvalidOpE.InvalidOp
-      | _, _ =>
-          Fitree.trigger InvalidOpE.InvalidOp
+  | Op.mk "toy.reshape" [t_name] [] [] _
+        (.fn (builtin.tensor D τ₁) (builtin.tensor D' τ₂)) =>
+      if H: τ₁ = τ₂
+        ∧ DimList.known D
+        ∧ DimList.known D'
+        ∧ DimList.prod D' = DimList.prod D then do
+        let t ← Fitree.trigger (SSAEnvE.Get (builtin.tensor D τ₁) t_name);
+        let t' ← Fitree.trigger (ToyOp.Reshape τ₁ D D'
+                H.2.1 H.2.2.1 H.2.2.2 t);
+        let t': RankedTensor D' τ₂ := cast (by rw [H.1]) t';
+        SSAEnv.set? (builtin.tensor D' τ₂) ret_name t'
+      else
+        Fitree.trigger InvalidOpE.InvalidOp
 
   | _ =>
       Fitree.trigger InvalidOpE.InvalidOp
 
 def toy_semantics_bbstmt:
-      BasicBlockStmt → Fitree (InvalidOpE +' SSAEnvE +' ToyOp) Unit
+      BasicBlockStmt builtin →
+      Fitree (InvalidOpE +' (SSAEnvE builtin) +' ToyOp) Unit
   | BasicBlockStmt.StmtAssign val _ op =>
       toy_semantics_op (some val) op
   | BasicBlockStmt.StmtOp op =>
@@ -107,7 +103,8 @@ def toy_semantics_bbstmt:
 -- TODO: toy_semantics_bb: handle basic block arguments
 @[simp]
 def toy_semantics_bb:
-      BasicBlock → Fitree (InvalidOpE +' SSAEnvE +' ToyOp) Unit
+      BasicBlock builtin →
+      Fitree (InvalidOpE +' (SSAEnvE builtin) +' ToyOp) Unit
   | BasicBlock.mk name args [] =>
       Fitree.ret ()
   | BasicBlock.mk name args (op1::ops) =>
@@ -132,8 +129,8 @@ def interp_toy {E} (t: Fitree (ToyOp +' E) R): Fitree E R :=
   interp (case_ ToyOp.handle (fun T => @Fitree.trigger E E T _)) t
 
 @[simp]
-def run_toy (t: Fitree (InvalidOpE +' SSAEnvE +' ToyOp) Unit) (env: SSAEnv):
-    Fitree PVoid (Unit × SSAEnv) :=
+def run_toy (t: Fitree (InvalidOpE +' SSAEnvE builtin +' ToyOp) Unit)
+    (env: SSAEnv builtin): Fitree PVoid (Unit × SSAEnv builtin) :=
   interp ToyOp.handle (interp_ssa (interp_invalid t sorry) env)
 
 /-
@@ -152,43 +149,19 @@ and finally the Toy operations themselves.
 ### Examples and testing
 -/
 
--- The following extends #reduce with a (skipProofs := true/false) parameter
--- to not reduce proofs in the kernel. Reducing proofs would cause constant
--- timeouts, and proofs are used implicitly through well-founded induction for
--- mutual definitions.
--- See: https://leanprover.zulipchat.com/#narrow/stream/270676-lean4/topic/Repr.20instance.20for.20functions/near/276504682
-
-open Lean
-open Lean.Parser.Term
-open Lean.Elab.Command
-open Lean.Elab
-open Lean.Meta
-
-elab "#reduce " skipProofs:group(atomic("(" &"skipProofs") " := " (trueVal <|> falseVal) ")") term:term : command =>
-  let skipProofs := skipProofs[3].isOfKind ``trueVal
-  withoutModifyingEnv <| runTermElabM (some `_check) fun _ => do
-    -- dbg_trace term
-    let e ← Term.elabTerm term none
-    Term.synthesizeSyntheticMVarsNoPostponing
-    let (e, _) ← Term.levelMVarToParam (← instantiateMVars e)
-    withTheReader Core.Context (fun ctx => { ctx with options := ctx.options.setBool `smartUnfolding false }) do
-      let e ← withTransparency (mode := TransparencyMode.all) <| reduce e (skipProofs := skipProofs) (skipTypes := false)
-      logInfo e
-
----
-
-def transpose_stmt := [mlir_bb_stmt|
+-- TODO: Can we infer the builtin in there?
+def transpose_stmt: BasicBlockStmt builtin := [mlir_bb_stmt|
   %t2 = "toy.transpose"(%t1): tensor<2×4×i32> -> tensor<4×2×i32>
 ]
 
-def constant_stmt := [mlir_bb_stmt|
+def constant_stmt: BasicBlockStmt builtin := [mlir_bb_stmt|
   %t = "toy.constant"() {value=dense<[[1,2],[3,4]]>: tensor<2×2×i32>}:
     () -> tensor<2×2×i32>
 ]
 
 #reduce constant_stmt
 
-def double_transpose := [mlir_bb|
+def double_transpose: BasicBlock builtin := [mlir_bb|
   ^dbl:
     %t2 = "toy.transpose"(%t1): tensor<2×4×i32> -> tensor<4×2×i32>
     %t3 = "toy.transpose"(%t2): tensor<4×2×i32> -> tensor<2×4×i32>
@@ -204,15 +177,15 @@ def double_transpose := [mlir_bb|
   run_toy (toy_semantics_bbstmt constant_stmt) [[]]
 
 theorem double_transpose_correct:
-  ∀ (t1: RankedTensor Int [2,4]),
+  ∀ (t1: RankedTensor [.Known 2, .Known 4] (.int 32)),
     run_toy (toy_semantics_bb double_transpose)
-      [[("t1", ⟨MLIRTy.tensorRanked [2,4] (MLIRTy.int 32), t1⟩)]]
+      [[("t1", ⟨builtin.tensor [.Known 2, .Known 4] (.int 32), t1⟩)]]
     =
     Fitree.ret ((), [[
-      (SSAVal.SSAVal "t1", ⟨MLIRTy.tensorRanked [2,4] (MLIRTy.int 32), t1⟩),
-      (SSAVal.SSAVal "t2", ⟨MLIRTy.tensorRanked [4,2] (MLIRTy.int 32),
+      (SSAVal.SSAVal "t1", ⟨builtin.tensor [.Known 2, .Known 4] (.int 32), t1⟩),
+      (SSAVal.SSAVal "t2", ⟨builtin.tensor [.Known 4, .Known 2] (.int 32),
                            transpose t1⟩),
-      (SSAVal.SSAVal "t3", ⟨MLIRTy.tensorRanked [2,4] (MLIRTy.int 32), t1⟩)
+      (SSAVal.SSAVal "t3", ⟨builtin.tensor [.Known 2, .Known 4] (.int 32), t1⟩)
     ]]) := by
   intros t1
   unfold double_transpose
@@ -221,4 +194,3 @@ theorem double_transpose_correct:
   simp [interp_invalid]; simp_itree
   simp [interp_ssa]; simp_itree
   rw [transpose_involutive]
-  rfl
