git/opencompl/lean-mlir/MLIR/Semantics/SSAEnv.lean
@@ -3,7 +3,7 @@
 
 This file implements the SSA environment which maps variables names from
 different scopes to explicitly-typed values. It is, conceptually, a map
-`SSAVal → (α: MLIRTy) × α` for each scope.
+`SSAVal → (α: MLIRType δ) × α` for each scope.
 
 The main concern with such state is the definition, maintainance and use of the
 property that the values are defined only once, allowing us to study sections
@@ -27,18 +27,22 @@ care when proving the correction of transformations.
 
 import MLIR.Semantics.Fitree
 import MLIR.Semantics.Types
+import MLIR.Util.WriterT
 
 import MLIR.AST
 open MLIR.AST
 
+section
+variable {α σ: Type} {ε: σ → Type}
 
 -- SSAScope
 
-def SSAScope :=
-  List (SSAVal × (τ: MLIRTy) × τ.eval)
+def SSAScope (δ: Dialect α σ ε) :=
+  List (SSAVal × (τ: MLIRType δ) × τ.eval)
 
 @[simp]
-def SSAScope.get (name: SSAVal): SSAScope → (τ: MLIRTy) → Option τ.eval
+def SSAScope.get {δ: Dialect α σ ε} (name: SSAVal):
+  SSAScope δ → (τ: MLIRType δ) → Option τ.eval
   | [], _ => none
   | ⟨name', τ', v'⟩ :: l, τ =>
       if H: name' = name && τ' = τ then
@@ -46,8 +50,8 @@ def SSAScope.get (name: SSAVal): SSAScope → (τ: MLIRTy) → Option τ.eval
       else get name l τ
 
 @[simp]
-def SSAScope.set (name: SSAVal) (τ: MLIRTy) (v: τ.eval):
-      SSAScope → SSAScope
+def SSAScope.set {δ: Dialect α σ ε} (name: SSAVal) (τ: MLIRType δ) (v: τ.eval):
+  SSAScope δ → SSAScope δ
   | [] => [⟨name, τ, v⟩]
   | ⟨name', τ', v'⟩ :: l =>
       if name' = name
@@ -67,14 +71,15 @@ def SSAScope.maps (l: SSAScope) (name: SSAVal) (τ: MLIRTy) (v: τ.eval) :=
 
 -- SSAEnv
 
-def SSAEnv :=
-  List SSAScope
+def SSAEnv (δ: Dialect α σ ε) :=
+  List (SSAScope δ)
 
--- | An SSA environment with a single empty SSAScope
-def SSAEnv.empty: SSAEnv := [[]]
+-- An SSA environment with a single empty SSAScope
+def SSAEnv.empty {δ: Dialect α σ ε}: SSAEnv δ := [[]]
 
 @[simp]
-def SSAEnv.get (name: SSAVal) (τ: MLIRTy): SSAEnv → Option τ.eval
+def SSAEnv.get {δ: Dialect α σ ε} (name: SSAVal) (τ: MLIRType δ):
+  SSAEnv δ → Option τ.eval
   | [] => none
   | l :: s =>
       match l.get name τ with
@@ -82,7 +87,8 @@ def SSAEnv.get (name: SSAVal) (τ: MLIRTy): SSAEnv → Option τ.eval
       | some v => v
 
 @[simp]
-def SSAEnv.set (name: SSAVal) (τ: MLIRTy) (v: τ.eval): SSAEnv → SSAEnv
+def SSAEnv.set {δ: Dialect α σ ε} (name: SSAVal) (τ: MLIRType δ) (v: τ.eval):
+  SSAEnv δ → SSAEnv δ
   | [] => [] -- cannot happen in practice
   | l :: s => l.set name τ v :: s
 
@@ -96,143 +102,61 @@ instance: LE SSAEnv where
 
 -- Interactions manipulating the environment
 
-inductive SSAEnvE: Type u → Type _ where
-  | Get: (τ: MLIRTy) → [Inhabited τ.eval] → SSAVal → SSAEnvE (ULift τ.eval)
-  | Set: (τ: MLIRTy) → SSAVal → τ.eval → SSAEnvE PUnit
+inductive SSAEnvE (δ: Dialect α σ ε): Type → Type where
+  | Get: (τ: MLIRType δ) → [Inhabited τ.eval] → SSAVal → SSAEnvE δ τ.eval
+  | Set: (τ: MLIRType δ) → SSAVal → τ.eval → SSAEnvE δ Unit
 
 @[simp_itree]
-def SSAEnvE.handle {E}: SSAEnvE ~> StateT SSAEnv (Fitree E) :=
+def SSAEnvE.handle {E}: SSAEnvE δ ~> StateT (SSAEnv δ) (Fitree E) :=
   fun _ e env =>
     match e with
     | Get τ name =>
         match env.get name τ with
-        | some v => return (ULift.up v, env)
-        | none => return (ULift.up default, env)
+        | some v => return (v, env)
+        | none => return (default, env)
     | Set τ name v =>
         return (.unit, env.set name τ v)
 
+def SSAEnvE.handleLogged {E}: SSAEnvE δ ~> WriterT (StateT (SSAEnv δ) (Fitree E)) :=
+  fun _ e => do
+    let env <- WriterT.lift StateT.get
+    match e with
+    | Get τ name =>
+        match env.get name τ with
+        | some v => do
+            logWriterT s!"get {name} (={v}); "
+            return v
+        | none =>
+            logWriterT s!"get {name} (not found!); "
+            return default
+    | Set τ name v =>
+        logWriterT s!"set {name}={v}; "
+        WriterT.lift $ StateT.set (env.set name τ v)
+        return ()
+
 @[simp_itree]
-def SSAEnv.set? {E} [Member SSAEnvE E]
-    (τ: MLIRTy) (name?: Option SSAVal) (v: τ.eval): Fitree E Unit :=
+def SSAEnv.set? {E} {δ: Dialect α σ ε} [Member (SSAEnvE δ) E]
+    (τ: MLIRType δ) (name?: Option SSAVal) (v: τ.eval): Fitree E Unit :=
   match name? with
   | some name =>
       Fitree.trigger (SSAEnvE.Set τ name v)
   | none =>
       return ()
 
--- In-context handler interpreting (SSAEnvE +' E ~> E)
+-- Handlers
 
 @[simp_itree]
-private def stateT_defaultHandler E: E ~> StateT SSAEnv (Fitree E) :=
-  fun _ e m => do
-    let r <- Fitree.trigger e;
-    return (r, m)
+private def stateT_defaultHandler: E ~> StateT (SSAEnv δ) (Fitree E) :=
+  fun _ e => StateT.lift $ Fitree.trigger e
 
-def interp_ssa {E R} (t: Fitree (SSAEnvE +' E) R):
-    StateT SSAEnv (Fitree E) R :=
-  interp_state (case_ SSAEnvE.handle (stateT_defaultHandler E)) t
+@[simp_itree]
+private def writerT_defaultHandler: E ~> WriterT (StateT (SSAEnv δ) (Fitree E)) :=
+  fun _ e => WriterT.lift $ StateT.lift $ Fitree.trigger e
 
-structure WriterT (m: Type _ -> Type _) (a: Type _) where
-  val: m (a × String)
+def interp_ssa {E R} (t: Fitree (SSAEnvE δ +' E) R):
+    StateT (SSAEnv δ) (Fitree E) R :=
+  interp_state (case_ SSAEnvE.handle stateT_defaultHandler) t
 
-def WriterT.run (wm: WriterT m a ): m (a × String) := wm.val
-
-instance [Functor m]: Functor (WriterT m) where
-  map f w := { val := Functor.map (fun (a, log) => (f a, log)) w.val }
-
-instance [Pure m]: Pure (WriterT m) where
-  pure x := { val := pure (x, "") }
-
-instance [Monad m]: Seq (WriterT m) where
-   seq mx my :=
-     { val := do
-        let wx <- mx.val
-        let wy <- (my ()).val
-        let wb := wx.fst wy.fst
-        return (wb, wx.snd ++ wy.snd) }
-
-instance [Monad m] : SeqLeft (WriterT m) where
-   seqLeft mx my :=
-     { val := do
-        let wx <- mx.val
-        let wy <- (my ()).val
-        return (wx.fst, wx.snd ++ wy.snd) }
-
-instance [Monad m] : SeqRight (WriterT m) where
-   seqRight mx my :=
-     { val := do
-        let wx <- mx.val
-        let wy <- (my ()).val
-        return (wy.fst, wx.snd  ++ wy.snd ) }
-
-instance [Bind m] [Pure m]: Bind (WriterT m) where
-  bind wma a2wmb :=
-    let v := do
-      let (va, loga) <- wma.val
-      let wb <- (a2wmb va).val
-      let (vb, logb) := wb
-      return (vb, loga ++ logb)
-    { val := v }
-
-def WriterT.lift [Monad m] {α : Type u} (ma: m α): WriterT m α :=
-  { val := do let a <- ma; return (a, "") }
-
-
-instance [Monad m]: MonadLift m (WriterT m) where
-  monadLift := WriterT.lift
-
-instance : MonadFunctor m (WriterT m) := ⟨fun f mx => { val := f (mx.val) } ⟩
-
-instance [Monad m] : Applicative (WriterT m) where
-  pure := Pure.pure
-  seqLeft := SeqLeft.seqLeft
-  seqRight := SeqRight.seqRight
-
-instance [Monad m]: Monad (WriterT m) where
-  pure := Pure.pure
-  bind := Bind.bind
-  map  := Functor.map
-
-def logWriterT [Monad m] (s: String): WriterT.{u} m PUnit.{u+1} :=
-  { val := pure (.unit, s) }
-
-
-
--- |
--- def SSAEnvE.handleLogged {E} {R: Type} (e: SSAEnvE R):  WriterT (StateT SSAEnv (Fitree E)) R := do
-def SSAEnvE.handleLogged (E: Type -> Type _) (R: Type): SSAEnvE ~>  WriterT (StateT SSAEnv (Fitree E)) :=
-  fun R e => do
-    let env <- WriterT.lift $ StateT.get
-    match e with
-    | Get τ name =>
-        logWriterT ("getting " ++ (ToString.toString name))
-        match env.get name τ with
-        | some v => do
-          let debugStr := match τ with | MLIRTy.int _ => toString v | _ => "unk"
-          logWriterT ("[val=" ++ debugStr ++ "];  ")
-          return ULift.up v
-        | none =>
-            logWriterT ("[val=none];  ")
-           return ULift.up default
-    | Set τ name v =>
-        logWriterT ("setting " ++ (ToString.toString name))
-        let debugStr := match τ with | MLIRTy.int _ => toString v | _ => "unk"
-        logWriterT ("[val=" ++ debugStr ++ "];  ")
-        WriterT.lift $ StateT.set (env.set name τ v)
-        return .unit
-
--- private def handleUnkLogged {E: Type -> Type _} {R: Type} (e: E R): WriterT (StateT SSAEnv (Fitree E)) R := do
-def handleUnkLogged (E: Type -> Type _): E ~> WriterT (StateT SSAEnv (Fitree E)) :=
-  fun R e => do
-    let r <- @Fitree.trigger E E _ _  e; -- TODO: understand precisely what this means
-    return r
-
--- Interpretation into the writer monad
-def interp_writer [Monad M] {E} (h: E ~> WriterT M):
-    forall ⦃R⦄, Fitree E R → WriterT M R := interp h
-
-def interp_ssa_logged {E R} (t: Fitree (SSAEnvE +' E) R):
-    WriterT (StateT SSAEnv (Fitree E)) R :=
-  let x := (case_ (SSAEnvE.handleLogged E R) (handleUnkLogged E))
-  let y := interp_writer x t
-  y
+def interp_ssa_logged {E R} (t: Fitree (SSAEnvE δ +' E) R):
+    WriterT (StateT (SSAEnv δ) (Fitree E)) R :=
+  interp_writer (case_ SSAEnvE.handleLogged writerT_defaultHandler) t
